WIP accessors

src/lowparse/LowParse.Low.Base.fst
@@ -337,740 +337,7 @@ let valid_facts
 = ()
 
 
-(* Accessors for reading only (no in-place serialization yet) *)
-
-noeq
-type clens (#t1: Type) (clens_cond: t1 -> GTot Type0) (t2: Type) = {
-  clens_get: (x1: t1) -> Ghost t2 (requires (clens_cond x1)) (ensures (fun _ -> True));
-(*  
-  clens_put: (x1: t1) -> t2 -> Ghost t1 (requires (clens_cond x1)) (ensures (fun x1' -> clens_cond x1'));
-  clens_get_put: (x1: t1) -> (x2: t2) -> Lemma (requires (clens_cond x1)) (ensures (clens_get (clens_put x1 x2) == x2));
-  clens_put_put: (x1: t1) -> (x2: t2) -> (x2' : t2) -> Lemma (requires (clens_cond x1)) (ensures (clens_put (clens_put x1 x2) x2' == clens_put x1 x2'));
-  clens_put_get: (x1: t1) -> Lemma (requires (clens_cond x1)) (ensures (clens_put x1 (clens_get x1) == x1));
-*)
-}
-
-(*
-let clens_get_put'
-  (#t1: Type) (#clens_cond: t1 -> GTot Type0) (#t2: Type) (l: clens clens_cond t2)
-  (x1: t1) (x2: t2)
-: Lemma
-  (requires (clens_cond x1))
-  (ensures (l.clens_get (l.clens_put x1 x2) == x2))
-  [SMTPat (l.clens_get (l.clens_put x1 x2))]
-= l.clens_get_put x1 x2
-
-let clens_put_put'
-  (#t1: Type) (#clens_cond: t1 -> GTot Type0) (#t2: Type) (l: clens clens_cond t2)
-  (x1: t1) (x2: t2) (x2' : t2)
-: Lemma
-  (requires (clens_cond x1))
-  (ensures (l.clens_put (l.clens_put x1 x2) x2' == l.clens_put x1 x2'))
-  [SMTPat (l.clens_put (l.clens_put x1 x2) x2')]
-= l.clens_put_put x1 x2 x2'
-
-let clens_put_get'
-  (#t1: Type) (#clens_cond: t1 -> GTot Type0) (#t2: Type) (l: clens clens_cond t2)
-  (x1: t1)
-: Lemma
-  (requires (clens_cond x1))
-  (ensures (l.clens_put x1 (l.clens_get x1) == x1))
-  [SMTPat (l.clens_put x1 (l.clens_get x1))]
-= l.clens_put_get x1
-
-abstract
-let clens_disjoint_l
-  (#t0: Type)
-  (#clens_cond2: t0 -> GTot Type0)
-  (#clens_cond3: t0 -> GTot Type0)
-  (#t2 #t3: Type)
-  (l2: clens clens_cond2 t2)
-  (l3: clens clens_cond3 t3)
-: GTot Type0
-= (forall (x0: t0) (x2: t2) . (clens_cond2 x0 /\ clens_cond3 x0) ==> 
-  (let x0' = l2.clens_put x0 x2 in clens_cond3 x0' /\ l3.clens_get x0' == l3.clens_get x0))
-
-abstract
-let clens_disjoint_l_elim
-  (#t0: Type)
-  (#clens_cond2: t0 -> GTot Type0)
-  (#clens_cond3: t0 -> GTot Type0)
-  (#t2 #t3: Type)
-  (l2: clens clens_cond2 t2)
-  (l3: clens clens_cond3 t3)
-  (x0: t0) (x2: t2)
-: Lemma
-  (requires (clens_disjoint_l l2 l3 /\ clens_cond2 x0 /\ clens_cond3 x0))
-  (ensures (let x0' = l2.clens_put x0 x2 in clens_cond3 x0' /\ l3.clens_get x0' == l3.clens_get x0))
-  [SMTPat (l3.clens_get (l2.clens_put x0 x2))]
-= ()
-
-abstract
-let clens_disjoint_l_intro
-  (#t0: Type)
-  (#clens_cond2: t0 -> GTot Type0)
-  (#clens_cond3: t0 -> GTot Type0)
-  (#t2 #t3: Type)
-  (l2: clens clens_cond2 t2)
-  (l3: clens clens_cond3 t3)
-  (lem: (
-    (x0: t0) ->
-    (x2: t2) ->
-    Lemma
-    (requires (clens_cond2 x0 /\ clens_cond3 x0))
-    (ensures (clens_cond2 x0 /\ clens_cond3 x0 /\ (let x0' = l2.clens_put x0 x2 in clens_cond3 x0' /\ l3.clens_get x0' == l3.clens_get x0)))
-  ))
-: Lemma
-  (clens_disjoint_l l2 l3)
-= let lem'
-    (x0: t0)
-    (x2: t2)
-  : Lemma
-    ((clens_cond2 x0 /\ clens_cond3 x0) ==>
-    (ensures (clens_cond2 x0 /\ clens_cond3 x0 /\ (let x0' = l2.clens_put x0 x2 in clens_cond3 x0' /\ l3.clens_get x0' == l3.clens_get x0))))
-  = Classical.move_requires (lem x0) x2
-  in
-  Classical.forall_intro_2 lem'
-
-let clens_disjoint
-  (#t0: Type)
-  (#clens_cond2: t0 -> GTot Type0)
-  (#clens_cond3: t0 -> GTot Type0)
-  (#t2 #t3: Type)
-  (l2: clens clens_cond2 t2)
-  (l3: clens clens_cond3 t3)
-: GTot Type0
-= clens_disjoint_l l2 l3 /\ clens_disjoint_l l3 l2
-
-let clens_disjoint_sym
-  (#t0: Type)
-  (#clens_cond2: t0 -> GTot Type0)
-  (#clens_cond3: t0 -> GTot Type0)
-  (#t2 #t3: Type)
-  (l2: clens clens_cond2 t2)
-  (l3: clens clens_cond3 t3)
-: Lemma
-  (clens_disjoint l2 l3 <==> clens_disjoint l3 l2)
-  [SMTPat (clens_disjoint l2 l3)]
-= ()
-*)
-
-let clens_compose_cond
-  (#t1: Type)
-  (#clens_cond1: t1 -> GTot Type0)
-  (#t2: Type)
-  (l12: clens clens_cond1 t2)
-  (clens_cond2: t2 -> GTot Type0)
-  (x1: t1)
-: GTot Type0
-= clens_cond1 x1 /\
-  clens_cond2 (l12.clens_get x1)
-
-let clens_compose
-  (#t1: Type)
-  (#clens_cond1: t1 -> GTot Type0)
-  (#t2: Type)
-  (#clens_cond2: t2 -> GTot Type0)
-  (#t3: Type)
-  (l12: clens clens_cond1 t2)
-  (l23: clens clens_cond2 t3)
-: Tot (clens (clens_compose_cond l12 clens_cond2) t3)
-= {
-  clens_get = (fun x1 -> l23.clens_get (l12.clens_get x1));
-(*  
-  clens_put = (fun x1 x3 ->
-    let x2' = l23.clens_put (l12.clens_get x1) x3 in
-    let x1' = l12.clens_put x1 x2' in
-    x1'
-  );
-  clens_get_put = (fun x1 x3 -> ());
-  clens_put_put = (fun x1 x3 x3' -> ());
-  clens_put_get = (fun x1 -> ());
-*)
-}
-
-(*
-abstract
-let clens_disjoint_compose
-  (#t0: Type)
-  (#clens_cond2: t0 -> GTot Type0)
-  (#clens_cond3: t0 -> GTot Type0)
-  (#t2 #t3: Type)
-  (l2: clens clens_cond2 t2)
-  (l3: clens clens_cond3 t3)
-  (#clens_cond3': t3 -> GTot Type0)
-  (#t3' : Type)
-  (l3' : clens clens_cond3' t3')
-: Lemma
-  (requires (clens_disjoint l2 l3))
-  (ensures (clens_disjoint l2 (clens_compose l3 l3')))
-  [SMTPat (clens_disjoint l2 (clens_compose l3 l3'))]
-= ()
-*)
-
-let gaccessor_pre
-  (#k1: parser_kind)
-  (#t1: Type)
-  (p1: parser k1 t1)
-  (#k2: parser_kind)
-  (#t2: Type)
-  (p2: parser k2 t2)
-  (#pre: t1 -> GTot Type0)
-  (cl: clens pre t2)
-  (sl: bytes)
-: GTot Type0
-= match parse p1 sl with
-  | Some (x1, consumed) -> (consumed <: nat) == Seq.length sl /\ pre x1
-  | _ -> False
-
-let gaccessor_post
-  (#k1: parser_kind)
-  (#t1: Type)
-  (p1: parser k1 t1)
-  (#k2: parser_kind)
-  (#t2: Type)
-  (p2: parser k2 t2)
-  (#pre: t1 -> GTot Type0)
-  (cl: clens pre t2)
-  (sl: bytes)
-  (res : nat & nat)
-: GTot Type0
-= let (pos', len) = res in
-  pos' + len <= Seq.length sl /\
-  begin match parse p1 sl with
-  | Some (x1, consumed1) ->
-    begin match parse p2 (Seq.slice sl pos' (pos' + len)) with
-    | Some (x2, consumed2) ->
-      pre x1 /\
-      x2 == cl.clens_get x1 /\
-      pos' + consumed2 <= consumed1 /\
-      consumed2 == len
-    | _ -> False
-    end
-  | _ -> False
-  end
-
-let gaccessor
-  (#k1: parser_kind)
-  (#t1: Type)
-  (p1: parser k1 t1)
-  (#k2: parser_kind)
-  (#t2: Type)
-  (p2: parser k2 t2)
-  (#pre: t1 -> GTot Type0)
-  (cl: clens pre t2)
-: Tot Type
-= (sl: bytes) ->
-  Ghost (nat & nat)
-  (requires (gaccessor_pre p1 p2 cl sl))
-  (ensures (fun pos' -> gaccessor_post p1 p2 cl sl pos'))
-
-abstract
-let gaccessors_disjoint
-  (#k1: parser_kind)
-  (#t1: Type)
-  (#p1: parser k1 t1)
-  (#k2: parser_kind)
-  (#t2: Type)
-  (#p2: parser k2 t2)
-  (#pre2: t1 -> GTot Type0)
-  (#cl2: clens pre2 t2)
-  (g2: gaccessor p1 p2 cl2)
-  (#k3: parser_kind)
-  (#t3: Type)
-  (#p3: parser k3 t3)
-  (#pre3: t1 -> GTot Type0)
-  (#cl3: clens pre3 t3)
-  (g3: gaccessor p1 p3 cl3)
-: GTot Type0
-= // clens_disjoint cl2 cl3 /\
-  (forall (sl: bytes) . (
-     match parse p1 sl with
-     | Some (x1, consumed1) -> pre2 x1 /\ pre3 x1 /\ consumed1 == Seq.length sl
-     | _ -> False
-   ) ==> (
-   let (pos2, consumed2) = g2 sl in
-   let (pos3, consumed3) = g3 sl in
-   pos2 + consumed2 <= pos3 \/ pos3 + consumed3 <= pos2
-  ))
-
-(*
-abstract
-let gaccessors_disjoint_clens_disjoint
-  (#k1: parser_kind)
-  (#t1: Type)
-  (#p1: parser k1 t1)
-  (#k2: parser_kind)
-  (#t2: Type)
-  (#p2: parser k2 t2)
-  (#pre2: t1 -> GTot Type0)
-  (#cl2: clens pre2 t2)
-  (g2: gaccessor p1 p2 cl2)
-  (#k3: parser_kind)
-  (#t3: Type)
-  (#p3: parser k3 t3)
-  (#pre3: t1 -> GTot Type0)
-  (#cl3: clens pre3 t3)
-  (g3: gaccessor p1 p3 cl3)
-: Lemma
-  (requires (gaccessors_disjoint g2 g3))
-  (ensures (clens_disjoint cl2 cl3))
-  [SMTPat (gaccessors_disjoint g2 g3)]
-= ()
-*)
-
-abstract
-let gaccessors_disjoint_elim
-  (#k1: parser_kind)
-  (#t1: Type)
-  (#p1: parser k1 t1)
-  (#k2: parser_kind)
-  (#t2: Type)
-  (#p2: parser k2 t2)
-  (#pre2: t1 -> GTot Type0)
-  (#cl2: clens pre2 t2)
-  (g2: gaccessor p1 p2 cl2)
-  (#k3: parser_kind)
-  (#t3: Type)
-  (#p3: parser k3 t3)
-  (#pre3: t1 -> GTot Type0)
-  (#cl3: clens pre3 t3)
-  (g3: gaccessor p1 p3 cl3)
-  (sl: bytes)
-: Lemma
-  (requires (gaccessors_disjoint g2 g3 /\ (
-     match parse p1 sl with
-     | Some (x1, consumed1) -> pre2 x1 /\ pre3 x1 /\ consumed1 == Seq.length sl
-     | _ -> False
-  )))
-  (ensures (
-    let (pos2, consumed2) = g2 sl in
-    let (pos3, consumed3) = g3 sl in
-    pos2 + consumed2 <= pos3 \/ pos3 + consumed3 <= pos2
-  ))
-= ()
-
-abstract
-let gaccessors_disjoint_intro
-  (#k1: parser_kind)
-  (#t1: Type)
-  (#p1: parser k1 t1)
-  (#k2: parser_kind)
-  (#t2: Type)
-  (#p2: parser k2 t2)
-  (#pre2: t1 -> GTot Type0)
-  (#cl2: clens pre2 t2)
-  (g2: gaccessor p1 p2 cl2)
-  (#k3: parser_kind)
-  (#t3: Type)
-  (#p3: parser k3 t3)
-  (#pre3: t1 -> GTot Type0)
-  (#cl3: clens pre3 t3)
-  (g3: gaccessor p1 p3 cl3)
-//  (clens_disj: squash (clens_disjoint cl2 cl3))
-  (lem: (
-    (sl: bytes) ->
-    Lemma
-    (requires (
-      match parse p1 sl with
-      | Some (x1, consumed1) -> pre2 x1 /\ pre3 x1 /\ consumed1 == Seq.length sl
-      | _ -> False
-    ))
-    (ensures ((
-      match parse p1 sl with
-      | Some (x1, consumed1) -> pre2 x1 /\ pre3 x1 /\ consumed1 == Seq.length sl
-      | _ -> False) /\ (
-      let (pos2, consumed2) = g2 sl in
-      let (pos3, consumed3) = g3 sl in
-      pos2 + consumed2 <= pos3 \/ pos3 + consumed3 <= pos2
-    )))
-  ))
-: Lemma
-  (gaccessors_disjoint g2 g3)
-= let lem'
-   (sl: bytes)
- : Lemma
-   ((
-     match parse p1 sl with
-     | Some (x1, consumed1) -> pre2 x1 /\ pre3 x1 /\ consumed1 == Seq.length sl
-     | _ -> False
-   ) ==> (
-   let (pos2, consumed2) = g2 sl in
-   let (pos3, consumed3) = g3 sl in
-   pos2 + consumed2 <= pos3 \/ pos3 + consumed3 <= pos2
-   ))
- = Classical.move_requires lem sl
- in
- Classical.forall_intro lem'
-
-let gaccessor_compose'
-  (#k1: parser_kind)
-  (#t1: Type)
-  (#p1: parser k1 t1)
-  (#k2: parser_kind)
-  (#t2: Type)
-  (#p2: parser k2 t2)
-  (#pre1: (t1 -> GTot Type0))
-  (#cl12: clens pre1 t2)
-  (a12: gaccessor p1 p2 cl12)
-  (#pre2: (t2 -> GTot Type0))
-  (#k3: parser_kind)
-  (#t3: Type)
-  (#p3: parser k3 t3)
-  (#cl23: clens pre2 t3)
-  (a23: gaccessor p2 p3 cl23)
-  (input: bytes)
-: Ghost (nat & nat)
-  (requires (gaccessor_pre p1 p3 (clens_compose cl12 cl23) input))
-  (ensures (fun pos' -> True))
-=
-  let (pos2, consumed2) = a12 input in
-  let input2 = Seq.slice input pos2 (pos2 + consumed2) in
-  let (pos3, consumed3) = a23 input2 in
-  (pos2 + pos3, consumed3)
-
-let gaccessor_compose_correct
-  (#k1: parser_kind)
-  (#t1: Type)
-  (#p1: parser k1 t1)
-  (#k2: parser_kind)
-  (#t2: Type)
-  (#p2: parser k2 t2)
-  (#pre1: (t1 -> GTot Type0))
-  (#cl12: clens pre1 t2)
-  (a12: gaccessor p1 p2 cl12)
-  (#pre2: (t2 -> GTot Type0))
-  (#k3: parser_kind)
-  (#t3: Type)
-  (#p3: parser k3 t3)
-  (#cl23: clens pre2 t3)
-  (a23: gaccessor p2 p3 cl23)
-  (input: bytes)
-: Lemma
-  (requires (gaccessor_pre p1 p3 (clens_compose cl12 cl23) input))
-  (ensures (gaccessor_post p1 p3 (clens_compose cl12 cl23) input (gaccessor_compose' a12 a23 input)))
-= ()
-
-let gaccessor_compose_
-  (#k1: parser_kind)
-  (#t1: Type)
-  (#p1: parser k1 t1)
-  (#k2: parser_kind)
-  (#t2: Type)
-  (#p2: parser k2 t2)
-  (#pre1: (t1 -> GTot Type0))
-  (#cl12: clens pre1 t2)
-  (a12: gaccessor p1 p2 cl12)
-  (#pre2: (t2 -> GTot Type0))
-  (#k3: parser_kind)
-  (#t3: Type)
-  (#p3: parser k3 t3)
-  (#cl23: clens pre2 t3)
-  (a23: gaccessor p2 p3 cl23)
-  (input: bytes)
-: Ghost (nat & nat)
-  (requires (gaccessor_pre p1 p3 (clens_compose cl12 cl23) input))
-  (ensures (fun pos' -> gaccessor_post p1 p3 (clens_compose cl12 cl23) input pos'))
-= gaccessor_compose_correct a12 a23 input;
-  gaccessor_compose' a12 a23 input
-
-let gaccessor_compose
-  (#k1: parser_kind)
-  (#t1: Type)
-  (#p1: parser k1 t1)
-  (#k2: parser_kind)
-  (#t2: Type)
-  (#p2: parser k2 t2)
-  (#pre1: (t1 -> GTot Type0))
-  (#cl12: clens pre1 t2)
-  (a12: gaccessor p1 p2 cl12)
-  (#pre2: (t2 -> GTot Type0))
-  (#k3: parser_kind)
-  (#t3: Type)
-  (#p3: parser k3 t3)
-  (#cl23: clens pre2 t3)
-  (a23: gaccessor p2 p3 cl23)
-: Tot (gaccessor p1 p3 (clens_compose cl12 cl23))
-= gaccessor_compose_ a12 a23
-
-let slice_access'
-  (h: HS.mem)
-  (#k1: parser_kind)
-  (#t1: Type)
-  (#p1: parser k1 t1)
-  (#k2: parser_kind)
-  (#t2: Type)
-  (#p2: parser k2 t2)
-  (#pre: t1 -> GTot Type0)
-  (#cl: clens pre t2)
-  (g: gaccessor p1 p2 cl)
-  (sl: slice)
-  (pos: U32.t)
-: Ghost U32.t
-  (requires (
-    k1.parser_kind_subkind == Some ParserStrong /\
-    valid' p1 h sl pos /\
-    pre (contents' p1 h sl pos)
-  ))
-  (ensures (fun pos' -> True))
-= 
-  let small = B.as_seq h (B.gsub sl.base pos (U32.uint_to_t (content_length' p1 h sl pos))) in
-  let _ =
-    let large = B.as_seq h (B.gsub sl.base pos (sl.len `U32.sub` pos)) in
-    assert (no_lookahead_on p1 large small);
-    assert (injective_postcond p1 large small)
-  in
-  pos `U32.add` U32.uint_to_t (fst (g small))
-
-(* HERE *)
-
-abstract
-let slice_access
-  (h: HS.mem)
-  (#k1: parser_kind)
-  (#t1: Type)
-  (#p1: parser k1 t1)
-  (#k2: parser_kind)
-  (#t2: Type)
-  (#p2: parser k2 t2)
-  (#pre: t1 -> GTot Type0)
-  (#cl: clens pre t2)
-  (g: gaccessor p1 p2 cl)
-  (sl: slice)
-  (pos: U32.t)
-: Ghost U32.t
-  (requires (
-    k1.parser_kind_subkind == Some ParserStrong /\
-    k2.parser_kind_subkind == Some ParserStrong /\
-    valid p1 h sl pos /\
-    pre (contents p1 h sl pos)
-  ))
-  (ensures (fun pos' ->
-    valid p2 h sl pos' /\
-    contents p2 h sl pos' == cl.clens_get (contents p1 h sl pos) /\
-    // useful for framing
-    U32.v pos <= U32.v pos' /\
-    U32.v pos' + content_length p2 h sl pos' <= U32.v pos + content_length p1 h sl pos
-  ))
-= let res = slice_access' h g sl pos in
-//  let _ =
-    let input = B.as_seq h (B.gsub sl.base pos (U32.uint_to_t (content_length' p1 h sl pos))) in
-    let output_small = B.as_seq h (B.gsub sl.base res (U32.uint_to_t (snd (g input)))) in
-    let output_large = B.as_seq h (B.gsub sl.base res (sl.len `U32.sub` res)) in
-    assert (no_lookahead_on p2 output_small output_large);
-    assert (injective_postcond p2 output_small output_large);
-    admit ();
-//  in
-  res
-
-abstract
-let slice_access_eq
-  (h: HS.mem)
-  (#k1: parser_kind)
-  (#t1: Type)
-  (#p1: parser k1 t1)
-  (#k2: parser_kind)
-  (#t2: Type)
-  (#p2: parser k2 t2)
-  (#pre: t1 -> GTot Type0)
-  (#cl: clens pre t2)
-  (g: gaccessor p1 p2 cl)
-  (sl: slice)
-  (pos: U32.t)
-: Lemma
-  (requires (
-    k1.parser_kind_subkind == Some ParserStrong /\
-    k2.parser_kind_subkind == Some ParserStrong /\
-    valid p1 h sl pos /\
-    pre (contents p1 h sl pos)
-  ))
-  (ensures (
-    valid' p1 h sl pos /\
-    pre (contents' p1 h sl pos) /\
-    slice_access h g sl pos == slice_access' h g sl pos
-  ))
-= ()
-
-abstract
-let slice_access_frame
-  (h: HS.mem)
-  (#k1: parser_kind)
-  (#t1: Type)
-  (#p1: parser k1 t1)
-  (#k2: parser_kind)
-  (#t2: Type)
-  (#p2: parser k2 t2)
-  (#pre: t1 -> GTot Type0)
-  (#cl: clens pre t2)
-  (g: gaccessor p1 p2 cl)
-  (sl: slice)
-  (pos: U32.t)
-  (l: B.loc)
-  (h' : HS.mem)
-: Lemma
-  (requires (
-    valid p1 h sl pos /\
-    pre (contents p1 h sl pos) /\
-    B.modifies l h h' /\
-    B.loc_disjoint l (loc_slice_from sl pos)
-  ))
-  (ensures (
-    valid p1 h' sl pos /\
-    pre (contents p1 h' sl pos) /\
-    slice_access h' g sl pos == slice_access h g sl pos
-  ))
-  [SMTPatOr [
-    [SMTPat (slice_access h g sl pos); SMTPat (B.modifies l h h')];
-    [SMTPat (slice_access h' g sl pos); SMTPat (B.modifies l h h')];
-  ]]
-= ()
-
-inline_for_extraction
-let max_uint32 : U32.t = 4294967295ul
-
-let max_uint32_correct
-  (x: U32.t)
-: Lemma
-  (U32.v x <= U32.v max_uint32)
-= ()
-
-inline_for_extraction
-class validator_cls = {
-  // FIXME: ideally, the min bound on validator_max_length should not be a hard constant
-  validator_max_length: (u: U32.t { 4 <= U32.v u /\ U32.v u < U32.v max_uint32 } )
-}
-
-inline_for_extraction
-let validator [| validator_cls |] (#k: parser_kind) (#t: Type) (p: parser k t) : Tot Type =
-  (sl: slice) ->
-  (pos: U32.t) ->
-  HST.Stack U32.t
-  (requires (fun h -> live_slice h sl /\ U32.v pos <= U32.v sl.len /\ U32.v sl.len <= U32.v validator_max_length))
-  (ensures (fun h res h' ->
-    B.modifies B.loc_none h h' /\ (
-    if U32.v res <= U32.v validator_max_length
-    then
-      valid_pos p h sl pos res
-    else
-      (~ (valid p h sl pos))
-  )))
-
-inline_for_extraction
-let jumper
-  (#k: parser_kind)
-  (#t: Type)
-  (p: parser k t)
-: Tot Type
-= (sl: slice) ->
-  (pos: U32.t) ->
-  HST.Stack U32.t
-  (requires (fun h -> valid p h sl pos))
-  (ensures (fun h pos' h' ->
-    B.modifies B.loc_none h h' /\
-    U32.v pos + content_length p h sl pos == U32.v pos'
-  ))
-
-inline_for_extraction
-let accessor
-  (#k1: parser_kind)
-  (#t1: Type)
-  (#p1: parser k1 t1)
-  (#k2: parser_kind)
-  (#t2: Type)
-  (#p2: parser k2 t2)
-  (#pre: t1 -> GTot Type0)
-  (#cl: clens pre t2)
-  (g: gaccessor p1 p2 cl)
-: Tot Type
-= (sl: slice) ->
-  (pos: U32.t) ->
-  HST.Stack U32.t
-  (requires (fun h -> valid p1 h sl pos /\ pre (contents p1 h sl pos))) 
-  (ensures (fun h pos' h' ->
-    B.modifies B.loc_none h h' /\
-    pos' == slice_access h g sl pos
-  ))
-
-#push-options "--z3rlimit 16"
-
-inline_for_extraction
-let accessor_compose
-  (#k1: parser_kind)
-  (#t1: Type)
-  (#p1: parser k1 t1)
-  (#k2: parser_kind)
-  (#t2: Type)
-  (#p2: parser k2 t2)
-  (#pre1: (t1 -> GTot Type0))
-  (#cl12: clens pre1 t2)
-  (#a12: gaccessor p1 p2 cl12)
-  (a12' : accessor a12)
-  (#pre2: (t2 -> GTot Type0))
-  (#k3: parser_kind)
-  (#t3: Type)
-  (#p3: parser k3 t3)
-  (#cl23: clens pre2 t3)
-  (#a23: gaccessor p2 p3 cl23)
-  (a23' : accessor a23)
-: Tot (accessor (gaccessor_compose a12 a23))
-= fun input pos -> 
-  let pos2 = a12' input pos in
-  a23' input pos2
-
-#pop-options
-
-inline_for_extraction
-let leaf_reader
-  (#k: parser_kind)
-  (#t: Type)
-  (p: parser k t)
-: Tot Type
-= (sl: slice) ->
-  (pos: U32.t) ->
-  HST.Stack t
-  (requires (fun h -> valid p h sl pos))
-  (ensures (fun h res h' ->
-    B.modifies B.loc_none h h' /\
-    res == contents p h sl pos
-  ))
-
-inline_for_extraction
-let leaf_reader_ext
-  (#k1: parser_kind)
-  (#t: Type)
-  (#p1: parser k1 t)
-  (p32: leaf_reader p1)
-  (#k2: parser_kind)
-  (p2: parser k2 t)
-  (lem: (
-    (x: bytes) ->
-    Lemma
-    (parse p2 x == parse p1 x)
-  ))
-: Tot (leaf_reader p2)
-= fun sl pos ->
-  let h = HST.get () in
-  [@inline_let] let _ = lem (B.as_seq h (B.gsub sl.base pos (sl.len `U32.sub` pos))) in
-  p32 sl pos
-
-inline_for_extraction
-let leaf_writer_weak
-  (#k: parser_kind)
-  (#t: Type)
-  (#p: parser k t)
-  (s: serializer p)
-: Tot Type
-= (x: t) ->
-  (sl: slice) ->
-  (pos: U32.t) ->
-  HST.Stack U32.t
-  (requires (fun h -> live_slice h sl /\ U32.v pos <= U32.v sl.len /\ U32.v sl.len < U32.v max_uint32))
-  (ensures (fun h pos' h' ->
-    B.modifies (loc_slice_from sl pos) h h' /\ (
-    if pos' = max_uint32
-    then U32.v pos + serialized_length s x > U32.v sl.len
-    else valid_content_pos p h' sl pos x pos'
-  )))
+(* Case where we do not have the strong prefix property (e.g. lists): we need an extra length *)
 
 abstract
 let loc_slice_from_to
@@ -1137,189 +404,6 @@ let loc_slice_from_loc_slice_from_to_disjoint
   (ensures (B.loc_disjoint (loc_slice_from_to sl pos1 pos2) (loc_slice_from sl pos')))
   [SMTPat (B.loc_disjoint (loc_slice_from_to sl pos1 pos2) (loc_slice_from sl pos'))]
 = ()
-
-inline_for_extraction
-let leaf_writer_strong
-  (#k: parser_kind)
-  (#t: Type)
-  (#p: parser k t)
-  (s: serializer p)
-: Tot Type
-= (x: t) ->
-  (sl: slice) ->
-  (pos: U32.t) ->
-  HST.Stack U32.t
-  (requires (fun h -> live_slice h sl /\ U32.v pos + serialized_length s x <= U32.v sl.len))
-  (ensures (fun h pos' h' ->
-    B.modifies (loc_slice_from_to sl pos pos') h h' /\
-    valid_content_pos p h' sl pos x pos'
-  ))
-
-inline_for_extraction
-let serializer32
-  (#k: parser_kind)
-  (#t: Type)
-  (#p: parser k t)
-  (s: serializer p)
-: Tot Type
-= (x: t) ->
-  (b: buffer8) ->
-  HST.Stack U32.t
-  (requires (fun h -> B.live h b /\ Seq.length (serialize s x) <= B.length b))
-  (ensures (fun h len h' ->
-    Seq.length (serialize s x) == U32.v len /\ (
-    let b' = B.gsub b 0ul len in
-    B.modifies (B.loc_buffer b') h h' /\
-    B.live h b /\
-    B.as_seq h' b' `Seq.equal` serialize s x
-  )))
-
-inline_for_extraction
-let leaf_writer_strong_of_serializer32
-  (#k: parser_kind)
-  (#t: Type)
-  (#p: parser k t)
-  (#s: serializer p)
-  (s32: serializer32 s)
-  (u: squash (k.parser_kind_subkind == Some ParserStrong))
-: Tot (leaf_writer_strong s)
-= fun x input pos ->
-  let b = B.sub input.base pos (input.len `U32.sub` pos) in
-  let len = s32 x b in
-  let h = HST.get () in
-  [@inline_let] let pos' = pos `U32.add` len in
-  [@inline_let] let _ : squash (valid_content_pos p h input pos x pos') =
-    let small = B.as_seq h (B.gsub b 0ul len) in
-    let large = B.as_seq h b in
-    assert (no_lookahead_on p small large);
-    assert (injective_postcond p small large);
-    valid_facts p h input pos;
-    ()
-  in
-  pos'
-
-inline_for_extraction
-let leaf_writer_weak_of_strong_constant_size
-  (#k: parser_kind)
-  (#t: Type)
-  (#p: parser k t)
-  (#s: serializer p)
-  (s32: leaf_writer_strong s)
-  (sz: U32.t)
-  (u: squash (
-    k.parser_kind_high == Some k.parser_kind_low /\
-    k.parser_kind_low == U32.v sz /\
-    k.parser_kind_low < U32.v max_uint32
-  ))
-: Tot (leaf_writer_weak s)
-= fun x input pos ->
-  if (input.len `U32.sub` pos) `U32.lt` sz
-  then max_uint32
-  else s32 x input pos
-
-#set-options "--z3rlimit 16"
-
-inline_for_extraction
-let copy_strong
-  (#k: parser_kind)
-  (#t: Type)
-  (p: parser k t)
-  (src: slice) // FIXME: length is useless here
-  (spos spos' : U32.t)
-  (dst: slice)
-  (dpos: U32.t)
-: HST.Stack U32.t
-  (requires (fun h ->
-    k.parser_kind_subkind == Some ParserStrong /\
-    valid_pos p h src spos spos' /\ (
-    let clen = content_length p h src spos in
-    U32.v dpos + clen <= U32.v dst.len /\
-    live_slice h dst /\
-    B.loc_disjoint (loc_slice_from_to src spos spos') (loc_slice_from_to dst dpos (dpos `U32.add` (U32.uint_to_t clen)))
-  )))
-  (ensures (fun h dpos' h' ->
-    B.modifies (loc_slice_from_to dst dpos dpos') h h' /\
-    valid_content_pos p h' dst dpos (contents p h src spos) dpos'
-  ))
-= let h0 = HST.get () in
-  let len = spos' `U32.sub` spos in
-  let src' = B.sub src.base spos len in
-  let dst' = B.sub dst.base dpos len in
-  B.blit src' 0ul dst' 0ul len;
-  let h = HST.get () in
-  [@inline_let] let dpos' = dpos `U32.add` len in
-  assert (
-    B.modifies (loc_slice_from_to dst dpos dpos') h0 h
-  );
-  assert (no_lookahead_on p (B.as_seq h0 (B.gsub src.base spos (src.len `U32.sub` spos))) (B.as_seq h (B.gsub dst.base dpos (dst.len `U32.sub` dpos))));
-  assert (no_lookahead_on_postcond p (B.as_seq h0 (B.gsub src.base spos (src.len `U32.sub` spos))) (B.as_seq h (B.gsub dst.base dpos (dst.len `U32.sub` dpos))));
-  assert (injective_precond p (B.as_seq h0 (B.gsub src.base spos (src.len `U32.sub` spos))) (B.as_seq h (B.gsub dst.base dpos (dst.len `U32.sub` dpos))));  
-  dpos'
-
-#reset-options
-
-inline_for_extraction
-let copy_weak_with_length
-  (#k: parser_kind)
-  (#t: Type)
-  (p: parser k t)
-  (src: slice) // FIXME: length is useless here
-  (spos spos' : U32.t)
-  (dst: slice)
-  (dpos: U32.t)
-: HST.Stack U32.t
-  (requires (fun h ->
-    k.parser_kind_subkind == Some ParserStrong /\
-    valid_pos p h src spos spos' /\
-    live_slice h dst /\
-    U32.v dpos <= U32.v dst.len /\
-    U32.v dst.len < U32.v max_uint32 /\
-    B.loc_disjoint (loc_slice_from_to src spos spos') (loc_slice_from dst dpos)
-  ))
-  (ensures (fun h dpos' h' ->
-    B.modifies (loc_slice_from dst dpos) h h' /\ (
-    if dpos' = max_uint32
-    then
-      U32.v dpos + content_length p h src spos > U32.v dst.len
-    else
-      valid_content_pos p h' dst dpos (contents p h src spos) dpos'
-  )))
-= if (dst.len `U32.sub` dpos) `U32.lt` (spos' `U32.sub` spos)
-  then max_uint32
-  else copy_strong p src spos spos' dst dpos
-
-inline_for_extraction
-let copy_weak
-  (#k: parser_kind)
-  (#t: Type)
-  (p: parser k t)
-  (jmp: jumper p)
-  (src: slice)
-  (spos : U32.t)
-  (dst: slice)
-  (dpos: U32.t)
-: HST.Stack U32.t
-  (requires (fun h ->
-    k.parser_kind_subkind == Some ParserStrong /\
-    valid p h src spos /\
-    live_slice h dst /\
-    U32.v dpos <= U32.v dst.len /\
-    U32.v dst.len < U32.v max_uint32 /\
-    B.loc_disjoint (loc_slice_from src spos) (loc_slice_from dst dpos)
-  ))
-  (ensures (fun h dpos' h' ->
-    B.modifies (loc_slice_from dst dpos) h h' /\ (
-    if dpos' = max_uint32
-    then
-      U32.v dpos + content_length p h src spos > U32.v dst.len
-    else
-      valid_content_pos p h' dst dpos (contents p h src spos) dpos'
-  )))
-= let spos' = jmp src spos in
-  copy_weak_with_length p src spos spos' dst dpos
-
-
-(* Case where we do not have the strong prefix property (e.g. lists): we need an extra length *)
 
 let valid_exact'
   (#k: parser_kind)
@@ -1575,3 +659,988 @@ let valid_exact_ext_elim
   ))
 = assert (injective_precond p (B.as_seq h (B.gsub s1.base pos1 (pos1' `U32.sub` pos1))) (B.as_seq h (B.gsub s2.base pos2 (pos2' `U32.sub` pos2))));
   assert (injective_postcond p (B.as_seq h (B.gsub s1.base pos1 (pos1' `U32.sub` pos1))) (B.as_seq h (B.gsub s2.base pos2 (pos2' `U32.sub` pos2))))
+
+(* Accessors for reading only (no in-place serialization yet) *)
+
+noeq
+type clens (#t1: Type) (clens_cond: t1 -> GTot Type0) (t2: Type) = {
+  clens_get: (x1: t1) -> Ghost t2 (requires (clens_cond x1)) (ensures (fun _ -> True));
+(*  
+  clens_put: (x1: t1) -> t2 -> Ghost t1 (requires (clens_cond x1)) (ensures (fun x1' -> clens_cond x1'));
+  clens_get_put: (x1: t1) -> (x2: t2) -> Lemma (requires (clens_cond x1)) (ensures (clens_get (clens_put x1 x2) == x2));
+  clens_put_put: (x1: t1) -> (x2: t2) -> (x2' : t2) -> Lemma (requires (clens_cond x1)) (ensures (clens_put (clens_put x1 x2) x2' == clens_put x1 x2'));
+  clens_put_get: (x1: t1) -> Lemma (requires (clens_cond x1)) (ensures (clens_put x1 (clens_get x1) == x1));
+*)
+}
+
+(*
+let clens_get_put'
+  (#t1: Type) (#clens_cond: t1 -> GTot Type0) (#t2: Type) (l: clens clens_cond t2)
+  (x1: t1) (x2: t2)
+: Lemma
+  (requires (clens_cond x1))
+  (ensures (l.clens_get (l.clens_put x1 x2) == x2))
+  [SMTPat (l.clens_get (l.clens_put x1 x2))]
+= l.clens_get_put x1 x2
+
+let clens_put_put'
+  (#t1: Type) (#clens_cond: t1 -> GTot Type0) (#t2: Type) (l: clens clens_cond t2)
+  (x1: t1) (x2: t2) (x2' : t2)
+: Lemma
+  (requires (clens_cond x1))
+  (ensures (l.clens_put (l.clens_put x1 x2) x2' == l.clens_put x1 x2'))
+  [SMTPat (l.clens_put (l.clens_put x1 x2) x2')]
+= l.clens_put_put x1 x2 x2'
+
+let clens_put_get'
+  (#t1: Type) (#clens_cond: t1 -> GTot Type0) (#t2: Type) (l: clens clens_cond t2)
+  (x1: t1)
+: Lemma
+  (requires (clens_cond x1))
+  (ensures (l.clens_put x1 (l.clens_get x1) == x1))
+  [SMTPat (l.clens_put x1 (l.clens_get x1))]
+= l.clens_put_get x1
+
+abstract
+let clens_disjoint_l
+  (#t0: Type)
+  (#clens_cond2: t0 -> GTot Type0)
+  (#clens_cond3: t0 -> GTot Type0)
+  (#t2 #t3: Type)
+  (l2: clens clens_cond2 t2)
+  (l3: clens clens_cond3 t3)
+: GTot Type0
+= (forall (x0: t0) (x2: t2) . (clens_cond2 x0 /\ clens_cond3 x0) ==> 
+  (let x0' = l2.clens_put x0 x2 in clens_cond3 x0' /\ l3.clens_get x0' == l3.clens_get x0))
+
+abstract
+let clens_disjoint_l_elim
+  (#t0: Type)
+  (#clens_cond2: t0 -> GTot Type0)
+  (#clens_cond3: t0 -> GTot Type0)
+  (#t2 #t3: Type)
+  (l2: clens clens_cond2 t2)
+  (l3: clens clens_cond3 t3)
+  (x0: t0) (x2: t2)
+: Lemma
+  (requires (clens_disjoint_l l2 l3 /\ clens_cond2 x0 /\ clens_cond3 x0))
+  (ensures (let x0' = l2.clens_put x0 x2 in clens_cond3 x0' /\ l3.clens_get x0' == l3.clens_get x0))
+  [SMTPat (l3.clens_get (l2.clens_put x0 x2))]
+= ()
+
+abstract
+let clens_disjoint_l_intro
+  (#t0: Type)
+  (#clens_cond2: t0 -> GTot Type0)
+  (#clens_cond3: t0 -> GTot Type0)
+  (#t2 #t3: Type)
+  (l2: clens clens_cond2 t2)
+  (l3: clens clens_cond3 t3)
+  (lem: (
+    (x0: t0) ->
+    (x2: t2) ->
+    Lemma
+    (requires (clens_cond2 x0 /\ clens_cond3 x0))
+    (ensures (clens_cond2 x0 /\ clens_cond3 x0 /\ (let x0' = l2.clens_put x0 x2 in clens_cond3 x0' /\ l3.clens_get x0' == l3.clens_get x0)))
+  ))
+: Lemma
+  (clens_disjoint_l l2 l3)
+= let lem'
+    (x0: t0)
+    (x2: t2)
+  : Lemma
+    ((clens_cond2 x0 /\ clens_cond3 x0) ==>
+    (ensures (clens_cond2 x0 /\ clens_cond3 x0 /\ (let x0' = l2.clens_put x0 x2 in clens_cond3 x0' /\ l3.clens_get x0' == l3.clens_get x0))))
+  = Classical.move_requires (lem x0) x2
+  in
+  Classical.forall_intro_2 lem'
+
+let clens_disjoint
+  (#t0: Type)
+  (#clens_cond2: t0 -> GTot Type0)
+  (#clens_cond3: t0 -> GTot Type0)
+  (#t2 #t3: Type)
+  (l2: clens clens_cond2 t2)
+  (l3: clens clens_cond3 t3)
+: GTot Type0
+= clens_disjoint_l l2 l3 /\ clens_disjoint_l l3 l2
+
+let clens_disjoint_sym
+  (#t0: Type)
+  (#clens_cond2: t0 -> GTot Type0)
+  (#clens_cond3: t0 -> GTot Type0)
+  (#t2 #t3: Type)
+  (l2: clens clens_cond2 t2)
+  (l3: clens clens_cond3 t3)
+: Lemma
+  (clens_disjoint l2 l3 <==> clens_disjoint l3 l2)
+  [SMTPat (clens_disjoint l2 l3)]
+= ()
+*)
+
+let clens_compose_cond
+  (#t1: Type)
+  (#clens_cond1: t1 -> GTot Type0)
+  (#t2: Type)
+  (l12: clens clens_cond1 t2)
+  (clens_cond2: t2 -> GTot Type0)
+  (x1: t1)
+: GTot Type0
+= clens_cond1 x1 /\
+  clens_cond2 (l12.clens_get x1)
+
+let clens_compose
+  (#t1: Type)
+  (#clens_cond1: t1 -> GTot Type0)
+  (#t2: Type)
+  (#clens_cond2: t2 -> GTot Type0)
+  (#t3: Type)
+  (l12: clens clens_cond1 t2)
+  (l23: clens clens_cond2 t3)
+: Tot (clens (clens_compose_cond l12 clens_cond2) t3)
+= {
+  clens_get = (fun x1 -> l23.clens_get (l12.clens_get x1));
+(*  
+  clens_put = (fun x1 x3 ->
+    let x2' = l23.clens_put (l12.clens_get x1) x3 in
+    let x1' = l12.clens_put x1 x2' in
+    x1'
+  );
+  clens_get_put = (fun x1 x3 -> ());
+  clens_put_put = (fun x1 x3 x3' -> ());
+  clens_put_get = (fun x1 -> ());
+*)
+}
+
+(*
+abstract
+let clens_disjoint_compose
+  (#t0: Type)
+  (#clens_cond2: t0 -> GTot Type0)
+  (#clens_cond3: t0 -> GTot Type0)
+  (#t2 #t3: Type)
+  (l2: clens clens_cond2 t2)
+  (l3: clens clens_cond3 t3)
+  (#clens_cond3': t3 -> GTot Type0)
+  (#t3' : Type)
+  (l3' : clens clens_cond3' t3')
+: Lemma
+  (requires (clens_disjoint l2 l3))
+  (ensures (clens_disjoint l2 (clens_compose l3 l3')))
+  [SMTPat (clens_disjoint l2 (clens_compose l3 l3'))]
+= ()
+*)
+
+let gaccessor_pre
+  (#k1: parser_kind)
+  (#t1: Type)
+  (p1: parser k1 t1)
+  (#k2: parser_kind)
+  (#t2: Type)
+  (p2: parser k2 t2)
+  (#pre: t1 -> GTot Type0)
+  (cl: clens pre t2)
+  (sl: bytes)
+: GTot Type0
+= match parse p1 sl with
+  | Some (x1, consumed) -> (consumed <: nat) == Seq.length sl /\ pre x1
+  | _ -> False
+
+let gaccessor_post
+  (#k1: parser_kind)
+  (#t1: Type)
+  (p1: parser k1 t1)
+  (#k2: parser_kind)
+  (#t2: Type)
+  (p2: parser k2 t2)
+  (#pre: t1 -> GTot Type0)
+  (cl: clens pre t2)
+  (sl: bytes)
+  (res : nat & nat)
+: GTot Type0
+= let (pos', len) = res in
+  pos' + len <= Seq.length sl /\
+  begin match parse p1 sl with
+  | Some (x1, consumed1) ->
+    begin match parse p2 (Seq.slice sl pos' (pos' + len)) with
+    | Some (x2, consumed2) ->
+      pre x1 /\
+      x2 == cl.clens_get x1 /\
+      pos' + consumed2 <= consumed1 /\
+      consumed2 == len
+    | _ -> False
+    end
+  | _ -> False
+  end
+
+let gaccessor_post' 
+  (#k1: parser_kind)
+  (#t1: Type)
+  (p1: parser k1 t1)
+  (#k2: parser_kind)
+  (#t2: Type)
+  (p2: parser k2 t2)
+  (#pre: t1 -> GTot Type0)
+  (cl: clens pre t2)
+  (sl : bytes)
+  (res: nat & nat)
+: GTot Type0
+= 
+    let (pos', len') = res in pos' + len' <= Seq.length sl /\
+    (gaccessor_pre p1 p2 cl sl ==> gaccessor_post p1 p2 cl sl res)
+
+let gaccessor
+  (#k1: parser_kind)
+  (#t1: Type)
+  (p1: parser k1 t1)
+  (#k2: parser_kind)
+  (#t2: Type)
+  (p2: parser k2 t2)
+  (#pre: t1 -> GTot Type0)
+  (cl: clens pre t2)
+: Tot Type
+= (sl: bytes) ->
+  Ghost (nat & nat)
+  (requires True)
+  (ensures (fun res ->
+    gaccessor_post' p1 p2 cl sl res
+  ))
+
+abstract
+let gaccessors_disjoint
+  (#k1: parser_kind)
+  (#t1: Type)
+  (#p1: parser k1 t1)
+  (#k2: parser_kind)
+  (#t2: Type)
+  (#p2: parser k2 t2)
+  (#pre2: t1 -> GTot Type0)
+  (#cl2: clens pre2 t2)
+  (g2: gaccessor p1 p2 cl2)
+  (#k3: parser_kind)
+  (#t3: Type)
+  (#p3: parser k3 t3)
+  (#pre3: t1 -> GTot Type0)
+  (#cl3: clens pre3 t3)
+  (g3: gaccessor p1 p3 cl3)
+: GTot Type0
+= // clens_disjoint cl2 cl3 /\
+  (forall (sl: bytes) . (
+     match parse p1 sl with
+     | Some (x1, consumed1) -> pre2 x1 /\ pre3 x1 /\ consumed1 == Seq.length sl
+     | _ -> False
+   ) ==> (
+   let (pos2, consumed2) = g2 sl in
+   let (pos3, consumed3) = g3 sl in
+   pos2 + consumed2 <= pos3 \/ pos3 + consumed3 <= pos2
+  ))
+
+(*
+abstract
+let gaccessors_disjoint_clens_disjoint
+  (#k1: parser_kind)
+  (#t1: Type)
+  (#p1: parser k1 t1)
+  (#k2: parser_kind)
+  (#t2: Type)
+  (#p2: parser k2 t2)
+  (#pre2: t1 -> GTot Type0)
+  (#cl2: clens pre2 t2)
+  (g2: gaccessor p1 p2 cl2)
+  (#k3: parser_kind)
+  (#t3: Type)
+  (#p3: parser k3 t3)
+  (#pre3: t1 -> GTot Type0)
+  (#cl3: clens pre3 t3)
+  (g3: gaccessor p1 p3 cl3)
+: Lemma
+  (requires (gaccessors_disjoint g2 g3))
+  (ensures (clens_disjoint cl2 cl3))
+  [SMTPat (gaccessors_disjoint g2 g3)]
+= ()
+*)
+
+abstract
+let gaccessors_disjoint_elim
+  (#k1: parser_kind)
+  (#t1: Type)
+  (#p1: parser k1 t1)
+  (#k2: parser_kind)
+  (#t2: Type)
+  (#p2: parser k2 t2)
+  (#pre2: t1 -> GTot Type0)
+  (#cl2: clens pre2 t2)
+  (g2: gaccessor p1 p2 cl2)
+  (#k3: parser_kind)
+  (#t3: Type)
+  (#p3: parser k3 t3)
+  (#pre3: t1 -> GTot Type0)
+  (#cl3: clens pre3 t3)
+  (g3: gaccessor p1 p3 cl3)
+  (sl: bytes)
+: Lemma
+  (requires (gaccessors_disjoint g2 g3 /\ (
+     match parse p1 sl with
+     | Some (x1, consumed1) -> pre2 x1 /\ pre3 x1 /\ consumed1 == Seq.length sl
+     | _ -> False
+  )))
+  (ensures (
+    let (pos2, consumed2) = g2 sl in
+    let (pos3, consumed3) = g3 sl in
+    pos2 + consumed2 <= pos3 \/ pos3 + consumed3 <= pos2
+  ))
+= ()
+
+abstract
+let gaccessors_disjoint_intro
+  (#k1: parser_kind)
+  (#t1: Type)
+  (#p1: parser k1 t1)
+  (#k2: parser_kind)
+  (#t2: Type)
+  (#p2: parser k2 t2)
+  (#pre2: t1 -> GTot Type0)
+  (#cl2: clens pre2 t2)
+  (g2: gaccessor p1 p2 cl2)
+  (#k3: parser_kind)
+  (#t3: Type)
+  (#p3: parser k3 t3)
+  (#pre3: t1 -> GTot Type0)
+  (#cl3: clens pre3 t3)
+  (g3: gaccessor p1 p3 cl3)
+//  (clens_disj: squash (clens_disjoint cl2 cl3))
+  (lem: (
+    (sl: bytes) ->
+    Lemma
+    (requires (
+      match parse p1 sl with
+      | Some (x1, consumed1) -> pre2 x1 /\ pre3 x1 /\ consumed1 == Seq.length sl
+      | _ -> False
+    ))
+    (ensures ((
+      match parse p1 sl with
+      | Some (x1, consumed1) -> pre2 x1 /\ pre3 x1 /\ consumed1 == Seq.length sl
+      | _ -> False) /\ (
+      let (pos2, consumed2) = g2 sl in
+      let (pos3, consumed3) = g3 sl in
+      pos2 + consumed2 <= pos3 \/ pos3 + consumed3 <= pos2
+    )))
+  ))
+: Lemma
+  (gaccessors_disjoint g2 g3)
+= let lem'
+   (sl: bytes)
+ : Lemma
+   ((
+     match parse p1 sl with
+     | Some (x1, consumed1) -> pre2 x1 /\ pre3 x1 /\ consumed1 == Seq.length sl
+     | _ -> False
+   ) ==> (
+   let (pos2, consumed2) = g2 sl in
+   let (pos3, consumed3) = g3 sl in
+   pos2 + consumed2 <= pos3 \/ pos3 + consumed3 <= pos2
+   ))
+ = Classical.move_requires lem sl
+ in
+ Classical.forall_intro lem'
+
+let gaccessor_compose'
+  (#k1: parser_kind)
+  (#t1: Type)
+  (#p1: parser k1 t1)
+  (#k2: parser_kind)
+  (#t2: Type)
+  (#p2: parser k2 t2)
+  (#pre1: (t1 -> GTot Type0))
+  (#cl12: clens pre1 t2)
+  (a12: gaccessor p1 p2 cl12)
+  (#pre2: (t2 -> GTot Type0))
+  (#k3: parser_kind)
+  (#t3: Type)
+  (#p3: parser k3 t3)
+  (#cl23: clens pre2 t3)
+  (a23: gaccessor p2 p3 cl23)
+  (input: bytes)
+: Ghost (nat & nat)
+  (requires True)
+  (ensures (fun res ->
+    let (pos', len') = res in pos' + len' <= Seq.length input
+  ))
+=
+  let (pos2, consumed2) = a12 input in
+  let input2 = Seq.slice input pos2 (pos2 + consumed2) in
+  let (pos3, consumed3) = a23 input2 in
+  (pos2 + pos3, consumed3)
+
+let gaccessor_compose_correct
+  (#k1: parser_kind)
+  (#t1: Type)
+  (#p1: parser k1 t1)
+  (#k2: parser_kind)
+  (#t2: Type)
+  (#p2: parser k2 t2)
+  (#pre1: (t1 -> GTot Type0))
+  (#cl12: clens pre1 t2)
+  (a12: gaccessor p1 p2 cl12)
+  (#pre2: (t2 -> GTot Type0))
+  (#k3: parser_kind)
+  (#t3: Type)
+  (#p3: parser k3 t3)
+  (#cl23: clens pre2 t3)
+  (a23: gaccessor p2 p3 cl23)
+  (input: bytes)
+: Lemma
+  (gaccessor_pre p1 p3 (clens_compose cl12 cl23) input ==> gaccessor_post p1 p3 (clens_compose cl12 cl23) input (gaccessor_compose' a12 a23 input))
+= ()
+
+let gaccessor_compose_
+  (#k1: parser_kind)
+  (#t1: Type)
+  (#p1: parser k1 t1)
+  (#k2: parser_kind)
+  (#t2: Type)
+  (#p2: parser k2 t2)
+  (#pre1: (t1 -> GTot Type0))
+  (#cl12: clens pre1 t2)
+  (a12: gaccessor p1 p2 cl12)
+  (#pre2: (t2 -> GTot Type0))
+  (#k3: parser_kind)
+  (#t3: Type)
+  (#p3: parser k3 t3)
+  (#cl23: clens pre2 t3)
+  (a23: gaccessor p2 p3 cl23)
+  (input: bytes)
+: Ghost (nat & nat)
+  (requires True)
+  (ensures (fun res ->
+    gaccessor_post' p1 p3 (clens_compose cl12 cl23) input res
+  ))
+= gaccessor_compose_correct a12 a23 input;
+  gaccessor_compose' a12 a23 input
+
+let gaccessor_compose
+  (#k1: parser_kind)
+  (#t1: Type)
+  (#p1: parser k1 t1)
+  (#k2: parser_kind)
+  (#t2: Type)
+  (#p2: parser k2 t2)
+  (#pre1: (t1 -> GTot Type0))
+  (#cl12: clens pre1 t2)
+  (a12: gaccessor p1 p2 cl12)
+  (#pre2: (t2 -> GTot Type0))
+  (#k3: parser_kind)
+  (#t3: Type)
+  (#p3: parser k3 t3)
+  (#cl23: clens pre2 t3)
+  (a23: gaccessor p2 p3 cl23)
+: Tot (gaccessor p1 p3 (clens_compose cl12 cl23))
+= gaccessor_compose_ a12 a23
+
+let slice_access'
+  (h: HS.mem)
+  (#k1: parser_kind)
+  (#t1: Type)
+  (#p1: parser k1 t1)
+  (#k2: parser_kind)
+  (#t2: Type)
+  (#p2: parser k2 t2)
+  (#pre: t1 -> GTot Type0)
+  (#cl: clens pre t2)
+  (g: gaccessor p1 p2 cl)
+  (sl: slice)
+  (pos: U32.t)
+: Ghost U32.t
+  (requires (
+    valid' p1 h sl pos
+  ))
+  (ensures (fun pos' -> True))
+= 
+  let small = B.as_seq h (B.gsub sl.base pos (U32.uint_to_t (content_length' p1 h sl pos))) in
+  pos `U32.add` U32.uint_to_t (fst (g small))
+
+#push-options "--z3rlimit 16"
+
+abstract
+let slice_access
+  (h: HS.mem)
+  (#k1: parser_kind)
+  (#t1: Type)
+  (#p1: parser k1 t1)
+  (#k2: parser_kind)
+  (#t2: Type)
+  (#p2: parser k2 t2)
+  (#pre: t1 -> GTot Type0)
+  (#cl: clens pre t2)
+  (g: gaccessor p1 p2 cl)
+  (sl: slice)
+  (pos: U32.t)
+: Ghost U32.t
+  (requires (
+    k1.parser_kind_subkind == Some ParserStrong /\
+    k2.parser_kind_subkind == Some ParserStrong /\
+    valid p1 h sl pos /\
+    pre (contents p1 h sl pos)
+  ))
+  (ensures (fun pos' ->
+    valid p2 h sl pos' /\
+    contents p2 h sl pos' == cl.clens_get (contents p1 h sl pos) /\
+    // useful for framing
+    U32.v pos <= U32.v pos' /\
+    U32.v pos' + content_length p2 h sl pos' <= U32.v pos + content_length p1 h sl pos
+  ))
+= let res = slice_access' h g sl pos in
+  let _ =
+    let input_large = B.as_seq h (B.gsub sl.base pos (sl.len `U32.sub` pos)) in
+    let input_small = B.as_seq h (B.gsub sl.base pos (U32.uint_to_t (content_length' p1 h sl pos))) in
+    assert (no_lookahead_on p1 input_large input_small);
+    assert (injective_postcond p1 input_large input_small);
+    let output_small = B.as_seq h (B.gsub sl.base res (U32.uint_to_t (snd (g input_small)))) in
+    let output_large = B.as_seq h (B.gsub sl.base res (sl.len `U32.sub` res)) in
+    assert (no_lookahead_on p2 output_small output_large);
+    assert (no_lookahead_on_postcond p2 output_small output_large);
+    assert (injective_precond p2 output_small output_large);
+    assert (injective_postcond p2 output_small output_large)
+  in
+  res
+
+#pop-options
+
+abstract
+let slice_access_eq
+  (h: HS.mem)
+  (#k1: parser_kind)
+  (#t1: Type)
+  (#p1: parser k1 t1)
+  (#k2: parser_kind)
+  (#t2: Type)
+  (#p2: parser k2 t2)
+  (#pre: t1 -> GTot Type0)
+  (#cl: clens pre t2)
+  (g: gaccessor p1 p2 cl)
+  (sl: slice)
+  (pos: U32.t)
+: Lemma
+  (requires (
+    k1.parser_kind_subkind == Some ParserStrong /\
+    k2.parser_kind_subkind == Some ParserStrong /\
+    valid p1 h sl pos /\
+    pre (contents p1 h sl pos)
+  ))
+  (ensures (
+    valid' p1 h sl pos /\
+    pre (contents' p1 h sl pos) /\
+    slice_access h g sl pos == slice_access' h g sl pos
+  ))
+= ()
+
+#push-options "--z3rlimit 32"
+
+abstract
+let slice_access_eq_inv
+  (h: HS.mem)
+  (#k1: parser_kind)
+  (#t1: Type)
+  (#p1: parser k1 t1)
+  (#k2: parser_kind)
+  (#t2: Type)
+  (#p2: parser k2 t2)
+  (#pre: t1 -> GTot Type0)
+  (#cl: clens pre t2)
+  (g: gaccessor p1 p2 cl)
+  (sl: slice)
+  (pos: U32.t)
+: Lemma
+  (requires (
+    k1.parser_kind_subkind == Some ParserStrong /\
+    k2.parser_kind_subkind == Some ParserStrong /\
+    valid p1 h sl pos /\
+    pre (contents p1 h sl pos)
+  ))
+  (ensures (
+    let pos2 = slice_access h g sl pos in
+    g (B.as_seq h (B.gsub sl.base pos (U32.uint_to_t (content_length p1 h sl pos)))) ==
+      (U32.v pos2, content_length p2 h sl pos2)
+  ))
+= let res = slice_access h g sl pos in
+    let input_large = B.as_seq h (B.gsub sl.base pos (sl.len `U32.sub` pos)) in
+    let input_small = B.as_seq h (B.gsub sl.base pos (U32.uint_to_t (content_length p1 h sl pos))) in
+    assert (no_lookahead_on p1 input_large input_small);
+    assert (injective_postcond p1 input_large input_small);
+    let output_small = B.as_seq h (B.gsub sl.base res (U32.uint_to_t (snd (g input_small)))) in
+    let output_large = B.as_seq h (B.gsub sl.base res (sl.len `U32.sub` res)) in
+    assert (no_lookahead_on p2 output_small output_large);
+    assert (no_lookahead_on_postcond p2 output_small output_large);
+    assert (injective_precond p2 output_small output_large);
+    assert (injective_postcond p2 output_small output_large);
+//    assert (gaccessor_post p1 p2 cl input_small (U32.v res, content_length p2 h sl res));
+    assume (fst (g input_small) == U32.v res);
+    assume (snd (g input_small) == content_length p2 h sl res)
+
+abstract
+let slice_access_frame
+  (h: HS.mem)
+  (#k1: parser_kind)
+  (#t1: Type)
+  (#p1: parser k1 t1)
+  (#k2: parser_kind)
+  (#t2: Type)
+  (#p2: parser k2 t2)
+  (#pre: t1 -> GTot Type0)
+  (#cl: clens pre t2)
+  (g: gaccessor p1 p2 cl)
+  (sl: slice)
+  (pos: U32.t)
+  (l: B.loc)
+  (h' : HS.mem)
+: Lemma
+  (requires (
+    k1.parser_kind_subkind == Some ParserStrong /\
+    k2.parser_kind_subkind == Some ParserStrong /\
+    valid p1 h sl pos /\
+    pre (contents p1 h sl pos) /\
+    B.modifies l h h' /\
+    B.loc_disjoint l (loc_slice_from_to sl pos (get_valid_pos p1 h sl pos))
+  ))
+  (ensures (
+    valid p1 h' sl pos /\
+    pre (contents p1 h' sl pos) /\
+    slice_access h' g sl pos == slice_access h g sl pos
+  ))
+  [SMTPatOr [
+    [SMTPat (slice_access h g sl pos); SMTPat (B.modifies l h h')];
+    [SMTPat (slice_access h' g sl pos); SMTPat (B.modifies l h h')];
+  ]]
+= ()
+
+inline_for_extraction
+let accessor
+  (#k1: parser_kind)
+  (#t1: Type)
+  (#p1: parser k1 t1)
+  (#k2: parser_kind)
+  (#t2: Type)
+  (#p2: parser k2 t2)
+  (#pre: t1 -> GTot Type0)
+  (#cl: clens pre t2)
+  (g: gaccessor p1 p2 cl)
+: Tot Type
+= (sl: slice) ->
+  (pos: U32.t) ->
+  HST.Stack U32.t
+  (requires (fun h -> k1.parser_kind_subkind == Some ParserStrong /\ k2.parser_kind_subkind == Some ParserStrong /\ valid p1 h sl pos /\ pre (contents p1 h sl pos))) 
+  (ensures (fun h pos' h' ->
+    B.modifies B.loc_none h h' /\
+    pos' == slice_access h g sl pos
+  ))
+
+inline_for_extraction
+let accessor_compose
+  (#k1: parser_kind)
+  (#t1: Type)
+  (#p1: parser k1 t1)
+  (#k2: parser_kind)
+  (#t2: Type)
+  (#p2: parser k2 t2)
+  (#pre1: (t1 -> GTot Type0))
+  (#cl12: clens pre1 t2)
+  (#a12: gaccessor p1 p2 cl12)
+  (a12' : accessor a12)
+  (#pre2: (t2 -> GTot Type0))
+  (#k3: parser_kind)
+  (#t3: Type)
+  (#p3: parser k3 t3)
+  (#cl23: clens pre2 t3)
+  (#a23: gaccessor p2 p3 cl23)
+  (a23' : accessor a23)
+  (sq: squash (k2.parser_kind_subkind == Some ParserStrong))
+: Tot (accessor (gaccessor_compose a12 a23))
+= fun input pos ->
+  let h = HST.get () in
+  let pos2 = a12' input pos in
+  let pos3 = a23' input pos2 in
+  slice_access_eq_inv h a12 input pos;
+  slice_access_eq_inv h a23 input pos2;
+  slice_access_eq_inv h (gaccessor_compose a12 a23) input pos;
+  pos3
+
+(* Validators *)
+
+inline_for_extraction
+let max_uint32 : U32.t = 4294967295ul
+
+let max_uint32_correct
+  (x: U32.t)
+: Lemma
+  (U32.v x <= U32.v max_uint32)
+= ()
+
+inline_for_extraction
+class validator_cls = {
+  // FIXME: ideally, the min bound on validator_max_length should not be a hard constant
+  validator_max_length: (u: U32.t { 4 <= U32.v u /\ U32.v u < U32.v max_uint32 } )
+}
+
+inline_for_extraction
+let validator [| validator_cls |] (#k: parser_kind) (#t: Type) (p: parser k t) : Tot Type =
+  (sl: slice) ->
+  (pos: U32.t) ->
+  HST.Stack U32.t
+  (requires (fun h -> live_slice h sl /\ U32.v pos <= U32.v sl.len /\ U32.v sl.len <= U32.v validator_max_length))
+  (ensures (fun h res h' ->
+    B.modifies B.loc_none h h' /\ (
+    if U32.v res <= U32.v validator_max_length
+    then
+      valid_pos p h sl pos res
+    else
+      (~ (valid p h sl pos))
+  )))
+
+inline_for_extraction
+let jumper
+  (#k: parser_kind)
+  (#t: Type)
+  (p: parser k t)
+: Tot Type
+= (sl: slice) ->
+  (pos: U32.t) ->
+  HST.Stack U32.t
+  (requires (fun h -> valid p h sl pos))
+  (ensures (fun h pos' h' ->
+    B.modifies B.loc_none h h' /\
+    U32.v pos + content_length p h sl pos == U32.v pos'
+  ))
+
+inline_for_extraction
+let leaf_reader
+  (#k: parser_kind)
+  (#t: Type)
+  (p: parser k t)
+: Tot Type
+= (sl: slice) ->
+  (pos: U32.t) ->
+  HST.Stack t
+  (requires (fun h -> valid p h sl pos))
+  (ensures (fun h res h' ->
+    B.modifies B.loc_none h h' /\
+    res == contents p h sl pos
+  ))
+
+inline_for_extraction
+let leaf_reader_ext
+  (#k1: parser_kind)
+  (#t: Type)
+  (#p1: parser k1 t)
+  (p32: leaf_reader p1)
+  (#k2: parser_kind)
+  (p2: parser k2 t)
+  (lem: (
+    (x: bytes) ->
+    Lemma
+    (parse p2 x == parse p1 x)
+  ))
+: Tot (leaf_reader p2)
+= fun sl pos ->
+  let h = HST.get () in
+  [@inline_let] let _ = lem (B.as_seq h (B.gsub sl.base pos (sl.len `U32.sub` pos))) in
+  p32 sl pos
+
+inline_for_extraction
+let leaf_writer_weak
+  (#k: parser_kind)
+  (#t: Type)
+  (#p: parser k t)
+  (s: serializer p)
+: Tot Type
+= (x: t) ->
+  (sl: slice) ->
+  (pos: U32.t) ->
+  HST.Stack U32.t
+  (requires (fun h -> live_slice h sl /\ U32.v pos <= U32.v sl.len /\ U32.v sl.len < U32.v max_uint32))
+  (ensures (fun h pos' h' ->
+    B.modifies (loc_slice_from sl pos) h h' /\ (
+    if pos' = max_uint32
+    then U32.v pos + serialized_length s x > U32.v sl.len
+    else valid_content_pos p h' sl pos x pos'
+  )))
+
+inline_for_extraction
+let leaf_writer_strong
+  (#k: parser_kind)
+  (#t: Type)
+  (#p: parser k t)
+  (s: serializer p)
+: Tot Type
+= (x: t) ->
+  (sl: slice) ->
+  (pos: U32.t) ->
+  HST.Stack U32.t
+  (requires (fun h -> live_slice h sl /\ U32.v pos + serialized_length s x <= U32.v sl.len))
+  (ensures (fun h pos' h' ->
+    B.modifies (loc_slice_from_to sl pos pos') h h' /\
+    valid_content_pos p h' sl pos x pos'
+  ))
+
+inline_for_extraction
+let serializer32
+  (#k: parser_kind)
+  (#t: Type)
+  (#p: parser k t)
+  (s: serializer p)
+: Tot Type
+= (x: t) ->
+  (b: buffer8) ->
+  HST.Stack U32.t
+  (requires (fun h -> B.live h b /\ Seq.length (serialize s x) <= B.length b))
+  (ensures (fun h len h' ->
+    Seq.length (serialize s x) == U32.v len /\ (
+    let b' = B.gsub b 0ul len in
+    B.modifies (B.loc_buffer b') h h' /\
+    B.live h b /\
+    B.as_seq h' b' `Seq.equal` serialize s x
+  )))
+
+inline_for_extraction
+let leaf_writer_strong_of_serializer32
+  (#k: parser_kind)
+  (#t: Type)
+  (#p: parser k t)
+  (#s: serializer p)
+  (s32: serializer32 s)
+  (u: squash (k.parser_kind_subkind == Some ParserStrong))
+: Tot (leaf_writer_strong s)
+= fun x input pos ->
+  let b = B.sub input.base pos (input.len `U32.sub` pos) in
+  let len = s32 x b in
+  let h = HST.get () in
+  [@inline_let] let pos' = pos `U32.add` len in
+  [@inline_let] let _ : squash (valid_content_pos p h input pos x pos') =
+    let small = B.as_seq h (B.gsub b 0ul len) in
+    let large = B.as_seq h b in
+    assert (no_lookahead_on p small large);
+    assert (injective_postcond p small large);
+    valid_facts p h input pos;
+    ()
+  in
+  pos'
+
+inline_for_extraction
+let leaf_writer_weak_of_strong_constant_size
+  (#k: parser_kind)
+  (#t: Type)
+  (#p: parser k t)
+  (#s: serializer p)
+  (s32: leaf_writer_strong s)
+  (sz: U32.t)
+  (u: squash (
+    k.parser_kind_high == Some k.parser_kind_low /\
+    k.parser_kind_low == U32.v sz /\
+    k.parser_kind_low < U32.v max_uint32
+  ))
+: Tot (leaf_writer_weak s)
+= fun x input pos ->
+  if (input.len `U32.sub` pos) `U32.lt` sz
+  then max_uint32
+  else s32 x input pos
+
+#set-options "--z3rlimit 16"
+
+inline_for_extraction
+let copy_strong
+  (#k: parser_kind)
+  (#t: Type)
+  (p: parser k t)
+  (src: slice) // FIXME: length is useless here
+  (spos spos' : U32.t)
+  (dst: slice)
+  (dpos: U32.t)
+: HST.Stack U32.t
+  (requires (fun h ->
+    k.parser_kind_subkind == Some ParserStrong /\
+    valid_pos p h src spos spos' /\ (
+    let clen = content_length p h src spos in
+    U32.v dpos + clen <= U32.v dst.len /\
+    live_slice h dst /\
+    B.loc_disjoint (loc_slice_from_to src spos spos') (loc_slice_from_to dst dpos (dpos `U32.add` (U32.uint_to_t clen)))
+  )))
+  (ensures (fun h dpos' h' ->
+    B.modifies (loc_slice_from_to dst dpos dpos') h h' /\
+    valid_content_pos p h' dst dpos (contents p h src spos) dpos'
+  ))
+= let h0 = HST.get () in
+  let len = spos' `U32.sub` spos in
+  let src' = B.sub src.base spos len in
+  let dst' = B.sub dst.base dpos len in
+  B.blit src' 0ul dst' 0ul len;
+  let h = HST.get () in
+  [@inline_let] let dpos' = dpos `U32.add` len in
+  assert (
+    B.modifies (loc_slice_from_to dst dpos dpos') h0 h
+  );
+  assert (no_lookahead_on p (B.as_seq h0 (B.gsub src.base spos (src.len `U32.sub` spos))) (B.as_seq h (B.gsub dst.base dpos (dst.len `U32.sub` dpos))));
+  assert (no_lookahead_on_postcond p (B.as_seq h0 (B.gsub src.base spos (src.len `U32.sub` spos))) (B.as_seq h (B.gsub dst.base dpos (dst.len `U32.sub` dpos))));
+  assert (injective_precond p (B.as_seq h0 (B.gsub src.base spos (src.len `U32.sub` spos))) (B.as_seq h (B.gsub dst.base dpos (dst.len `U32.sub` dpos))));  
+  dpos'
+
+#reset-options
+
+inline_for_extraction
+let copy_weak_with_length
+  (#k: parser_kind)
+  (#t: Type)
+  (p: parser k t)
+  (src: slice) // FIXME: length is useless here
+  (spos spos' : U32.t)
+  (dst: slice)
+  (dpos: U32.t)
+: HST.Stack U32.t
+  (requires (fun h ->
+    k.parser_kind_subkind == Some ParserStrong /\
+    valid_pos p h src spos spos' /\
+    live_slice h dst /\
+    U32.v dpos <= U32.v dst.len /\
+    U32.v dst.len < U32.v max_uint32 /\
+    B.loc_disjoint (loc_slice_from_to src spos spos') (loc_slice_from dst dpos)
+  ))
+  (ensures (fun h dpos' h' ->
+    B.modifies (loc_slice_from dst dpos) h h' /\ (
+    if dpos' = max_uint32
+    then
+      U32.v dpos + content_length p h src spos > U32.v dst.len
+    else
+      valid_content_pos p h' dst dpos (contents p h src spos) dpos'
+  )))
+= if (dst.len `U32.sub` dpos) `U32.lt` (spos' `U32.sub` spos)
+  then max_uint32
+  else copy_strong p src spos spos' dst dpos
+
+inline_for_extraction
+let copy_weak
+  (#k: parser_kind)
+  (#t: Type)
+  (p: parser k t)
+  (jmp: jumper p)
+  (src: slice)
+  (spos : U32.t)
+  (dst: slice)
+  (dpos: U32.t)
+: HST.Stack U32.t
+  (requires (fun h ->
+    k.parser_kind_subkind == Some ParserStrong /\
+    valid p h src spos /\
+    live_slice h dst /\
+    U32.v dpos <= U32.v dst.len /\
+    U32.v dst.len < U32.v max_uint32 /\
+    B.loc_disjoint (loc_slice_from src spos) (loc_slice_from dst dpos)
+  ))
+  (ensures (fun h dpos' h' ->
+    B.modifies (loc_slice_from dst dpos) h h' /\ (
+    if dpos' = max_uint32
+    then
+      U32.v dpos + content_length p h src spos > U32.v dst.len
+    else
+      valid_content_pos p h' dst dpos (contents p h src spos) dpos'
+  )))
+= let spos' = jmp src spos in
+  copy_weak_with_length p src spos spos' dst dpos
+
